Alright. So let's just linear algebra the hell outta this question
Let $X_i$ be 1 if the student gets the question right and -z if the student gets the question wrong

<ul>
<li> $X_i = 1$ if the student gets the question right 
$ Pr(X*i = 1) = \frac{1}{4} $
	<li> $X_i = -z$ if the student gets the question wrong 
$ Pr(X_i = -z) = \frac{3}{4} $
</ul>
$ 0 = \sum*{k=1}^{25} ( 1 \cdot Pr(X*i = 1) ) + \sum*{k=1}^{25} ( -z \cdot Pr(X*i = -z) ) $ 
$ 0 = \sum*{k=1}^{25} ( 1 \cdot \frac{1}{4} ) + \sum_{k=1}^{25} ( -z \cdot \frac{3}{4} ) $ 
$ 0 = 25 \cdot ( 1 \cdot \frac{1}{4} ) + 25(-z \cdot \frac{3}{4}) $ 
$ 0 = 25 \cdot \frac{1}{4} - 25z \cdot \frac{3}{4} $ 
$ 0 = \frac{25}{4} - \frac{75z}{4} $ 
$ 0 = 25 - 75z $ 
$ 75z = 25 $ 
$ z = \frac{25}{75} $ 
$ z = \frac{1}{3} $
