Let's calculate $f(1)$ first \\
$f(1) = f(0) + 8 \cdot 1 - 2 $ \\
$f(1) = -17 + 8 - 2 $ \\
$f(1) = -11 $
\begin{enumerate}
\item $ f(n) = 3n^{2} - n - 17 $ \\
$ f(1) = 3 \cdot 1^2 - 1 - 17 $ \\
$ f(1) = 3 - 1 - 17 $ \\
$ f(1) = -15 $
\item $ f(n) = 3n^{2} + n - 17 $ \\
$ f(1) = 3 \cdot 1^2 + 1 - 17 $ \\
$ f(1) = 3 + 1 - 17 $ \\
$ f(1) = -13 $
\item $ f(n) = 4n^{2} - 2n - 17 $ \\
$ f(1) = 4 \cdot 1^2 - 2 - 17 $ \\
$ f(1) = 4 - 2 - 17 $ \\
$ f(1) = -15 $
\item $ f(n) = 4n^{2} + 2n - 17 $ \\
$ f(1) = 4 \cdot 1^2 + 2 - 17 $ \\
$ f(1) = 4 + 2 - 17 $ \\
$ f(1) = -11 $
\end{enumerate}
The correct answer is $ f(n) = 4n^{2} + 2n - 17 $ because it is the only one that gives the correct value for $ f(1) $
