First, we can calculate values of f$(1)$ and f$(2)$ to see if we can find a pattern.

$f(1) = f(0) + 10(0) - 6 = 7 + 10 - 6 = 11$

$f(2) = f(1) + 10(1) - 6 = 11 + 10 - 6 = 15$

<ul>
    <li> $f(n) = 4n^{2} - 2n + $ <br/> 
    $f(1) = 4{(1)}^{2} - 2(1) + 7 = 4 - 2 + 7 = 9$
    <li> $f(n) = 4n^{2} - n + 7$ <br/> 
    $f(1) = 4{(1)}^{2} - 1 + 7 = 4 - 1 + 7 = 10$
    <li> $f(n) = 5n^{2} - 2n + 7$ <br/> 
    $f(1) = 5{(1)}^{2} - 2(1) + 7 = 5 - 2 + 7 = 10$
    <li> $f(n) = 5n^{2} - n + 7$ <br/> 
    $f(1) = 5{(1)}^{2} - 1 + 7 = 5 - 1 + 7 = 11$
</ul>

Based on the pattern, we can see that $f(n) = 5n^{2} - n + 7$ is the correct answer
