Let's find the first few values of $ f(n) $
$ f(2) = 2 {( \frac{1}{2})}^{2} \cdot 2 = 1 $
$ f(3) = 2 {( \frac{2}{3})}^{2} \cdot 1 = \frac{8}{9} $

<ul>
    <li> $ \frac{2^{n}}{{(n-1)}^{2}} $ <br/> 
    $f(2) = \frac{2^{2}}{{(2-1)}^{2}} = 4 $
    <li> $ \frac{2^{n-1}}{n^{2}} $ <br/> 
    $f(2) = \frac{2^{1}}{2^{2}} = \frac{1}{2} $
    <li> $ \frac{2^{n}}{n^{2}} $ <br/> 
    $f(2) = \frac{2^{2}}{2^{2}} = 1 $ <br/> 
    $f(3) = \frac{2^{3}}{3^{2}} = \frac{8}{9} $
    <li> $ \frac{n^{2}}{2^{n}} $ <br/> 
    $f(2) = \frac{2^{2}}{2^{2}} = 1 $ <br/> 
    $f(3) = \frac{3^{2}}{2^{3}} = \frac{9}{8} $
</ul>
Thus, $ \frac{2^{n}}{n^{2}} $ is the correct answer.
