We can calculate values of $ f(1) $ and $ f(2) $ to see if we can find a pattern. \\
$ f(1) = \frac{1}{3} \cdot 7 = \frac{7}{3} $ \\
$ f(2) = \frac{2}{3} \cdot \frac{7}{3} = \frac{14}{9} $
\begin{enumerate}
\item $ f(n) = 7 \cdot \frac{n!}{3^{n}} $ \\
$ f(1) = 7 \cdot \frac{1!}{3^{1}} = 7 \cdot \frac{1}{3} = \frac{7}{3} $
$ f(2) = 7 \cdot \frac{2!}{3^{2}} = 7 \cdot \frac{2}{9} = \frac{14}{9} $
\item $ f(n) = 7^{n} \cdot \frac{n!}{3^{n}} $
$ f(1) = 7^{1} \cdot \frac{1!}{3^{1}} = 7 \cdot \frac{1}{3} = \frac{7}{3} $
$ f(2) = 7^{2} \cdot \frac{2!}{3^{2}} = 49 \cdot \frac{2}{9} = \frac{98}{9} $
\item $ f(n) = 7 \cdot \frac{(n+1)!}{3^{n}} $
$ f(1) = 7 \cdot \frac{2!}{3^{1}} = 7 \cdot \frac{2}{3} = \frac{14}{3} $
\item $ f(n) = 7^{n} \cdot \frac{(n+1)!}{3^{n}} $
$ f(1) = 7^{1} \cdot \frac{2!}{3^{1}} = 7 \cdot \frac{2}{3} = \frac{14}{3} $
\end{enumerate}
Thus, we know that $ f(n) = 7 \cdot \frac{n!}{3^{n}} $ is the correct answer.
