First, we can calculate values of f$(1)$, $f(2)$, and $f(3)$ to see if we can find a pattern. 
$f(1) = f(0) + 6(0) - 2 = 2 - 2 = 0$ 
$f(2) = f(1) + 6(1) - 2 = 0 + 6 - 2 = 4$
<ul>
<li> $f(n) = 3n^{2} - 5n + 2$
$f(1) = 3{(1)}^{2} - 5(1) + 2 = 3 - 5 + 2 = 0$
<li> $f(n) = 3n^{2} + 5n + 2$
$f(1) = 3{(1)}^{2} + 5(1) + 2 = 3 + 5 + 2 = 10$
<li> $f(n) = 2n^{2} - 5n + 2$
$f(1) = 2{(1)}^{2} - 5(1) + 2 = 2 - 5 + 2 = -1$
<li> $f(n) = 2n^{2} + 5n + 2$
$f(1) = 2{(1)}^{2} + 5(1) + 2 = 2 + 5 + 2 = 9$
</ul>
Therefore, we know that $f(n) = 3n^{2} - 5n + 2$ is the correct answer since it fits the pattern
