Let's calculate $ T(1) $
$ T(1) = 3 \cdot f(0) + 1 = 3 \cdot 2 + 1 = 7 $

<ul>
<li> $ T(n) = \frac{5}{2} \cdot 3^{n} - 1 $ <br/> 
$ T(1) = \frac{5}{2} \cdot 3^{1} - 1 = \frac{5}{2} \cdot 3 - 1 = \frac{15}{2} - 1 = \frac{13}{2} $
<li> $ T(n) = \frac{3}{2} \cdot 3^{n} - \frac{1}{2} $ <br/> 
$ T(1) = \frac{3}{2} \cdot 3^{1} - \frac{1}{2} = \frac{3}{2} \cdot 3 - \frac{1}{2} = \frac{9}{2} - \frac{1}{2} = 4 $
<li> $ T(n) = \frac{5}{2} \cdot 3^{n} - \frac{1}{2} $ <br/> 
$ T(1) = \frac{5}{2} \cdot 3^{1} - \frac{1}{2} = \frac{5}{2} \cdot 3 - \frac{1}{2} = \frac{15}{2} - \frac{1}{2} = 7 $
<li> None of the above
</ul>
We did it, everyone. The answer is C.
