<ul>
    <li> Let A be the event that we flip a head <br/>
    $ Pr(A) = \frac{1}{2} $
    <li> Let B be the event that we flip a tail <br/>
    $ Pr(B) = \frac{1}{2} $
</ul>

$ \mathbb{E}(X) = 2 \cdot \mathbb{E}(\text{number of heads}) - 3 \cdot \mathbb{E}(\text{number of tails}) $

$ \mathbb{E}(X) = 2 \cdot \sum\_{i=0}^{n} Pr(A) - 3 \cdot \sum\_{i=0}^{n} Pr(B) $

$ \mathbb{E}(X) = 2 \cdot n \cdot \frac{1}{2} - 3 \cdot n \cdot \frac{1}{2} $

$ \mathbb{E}(X) = n - \frac{3}{2}n $

$ \mathbb{E}(X) = \frac{2n}{2} - \frac{3n}{2} $

$ \mathbb{E}(X) = \frac{-n}{2} $
