Let's find the first few values of $ f(n) $ \\
$ f(2) = 2 {(\frac{1}{2})}^{2} \cdot 2 = 1 $ \\
$ f(3) = 2 {(\frac{2}{3})}^{2} \cdot 1 = \frac{8}{9} $
\begin{enumerate}
\item $ \frac{2^{n}}{{(n-1)}^{2}} $ \\
$f(2) = \frac{2^{2}}{{(2-1)}^{2}} = 4 $
\item $ \frac{2^{n-1}}{n^{2}} $ \\
$f(2) = \frac{2^{1}}{2^{2}} = \frac{1}{2} $
\item $ \frac{2^{n}}{n^{2}} $
$f(2) = \frac{2^{2}}{2^{2}} = 1 $ \\
$f(3) = \frac{2^{3}}{3^{2}} = \frac{8}{9} $
\item $ \frac{n^{2}}{2^{n}} $
$f(2) = \frac{2^{2}}{2^{2}} = 1 $ \\
$f(3) = \frac{3^{2}}{2^{3}} = \frac{9}{8} $
\end{enumerate}
Thus, $ \frac{2^{n}}{n^{2}} $ is the correct answer.
