We can first calculate values of f$(1)$ and f$(2)$ to see if we can find a pattern. \\
$f(1) = f(0) + 6(1) - 4 = 15 + 6 - 4 = 17$ \\
$f(2) = f(1) + 6(2) - 4 = 17 + 12 - 4 = 25$
\begin{enumerate}
\item $f(n) = 3n^{2} + 2n + 15$ \\
$f(1) = 3{(1)}^{2} + 2(1) + 15 = 3 + 2 + 15 = 20$
\item $f(n) = 3n^{2} - 2n + 15$ \\
$f(1) = 3{(1)}^{2} - 2(1) + 15 = 3 - 2 + 15 = 16$
\item $f(n) = 3n^{2} + n + 15$ \\
$f(1) = 3{(1)}^{2} + 1 + 15 = 3 + 1 + 15 = 19$
\item $f(n) = 3n^{2} - n + 15$ \\
$f(1) = 3{(1)}^{2} - 1 + 15 = 3 - 1 + 15 = 17$
\end{enumerate}
Therefore, we know that $f(n) = 3n^{2} - n + 15$ is the correct answer
