1. Let's calculat ethe first few values of $f(n)$ to see if we can find a pattern:

   $ f(1) = 3 \cdot f(0) + 1 = 3 \cdot 2 + 1 = 7 $

2. Let's see how the functions behave

   <ul>
       <li> $f(n) = \frac{5}{2} \cdot 3^n - 1$ <br/>
       $ f(1) = \frac{5}{2} \cdot 3^1 - 1 = \frac{5}{2} \cdot 3 - 1 = 7.5 - 1 = 6.5 $
       <li> $f(n) = \frac{3}{2} \cdot 3^n - \frac{1}{2}$ <br/>
       $ f(1) = \frac{3}{2} \cdot 3^1 - \frac{1}{2} = \frac{3}{2} \cdot 3 - \frac{1}{2} = 4.5 - 0.5 = 4 $
       <li> $f(n) = \frac{5}{2} \cdot 3^n - \frac{1}{2}$ <br/>
       $ f(1) = \frac{5}{2} \cdot 3^1 - \frac{1}{2} = \frac{5}{2} \cdot 3 - \frac{1}{2} = 7.5 - 0.5 = 7 $
   </ul>

   So the correct answer is the third option. $f(n) = \frac{5}{2} \cdot 3^n - \frac{1}{2}$
